Communication_Topology_Soundness.thy
@@ -1,0 +1,20 @@
+theory Communication_Topology_Soundness
+  imports 
+    Main 
+    Syntax Semantics 
+    Abstract_Value_Flow_Analysis Abstract_Value_Flow_Soundness
+    Communication_Topology_Analysis
+begin
+
+theorem topology_sound : "
+  \<lbrakk>
+    \<A> \<bind> e; 
+    [[] \<mapsto> <<e, empty, []>>] \<rightarrow>* \<E>';
+    \<E>' \<pi> = Some (<<e', \<rho>', \<kappa>'>>)
+  \<rbrakk> \<Longrightarrow>
+  \<langle>\<langle>\<rho>'\<rangle>\<rangle> \<sqsubseteq>\<^sub>t \<A>
+"
+ sorry
+
+
+end
